wip

lawyer/nonblocking/tokens/om_wfree_inst_tokens.v
@@ -2,29 +2,15 @@ From iris.proofmode Require Import tactics.
 From lawyer.examples Require Import orders_lib.
 From lawyer.obligations Require Import env_helpers obligations_model.
 From lawyer.nonblocking Require Import om_wfree_inst.
-From lawyer.nonblocking.tokens Require Import logrel_tok.
+From lawyer.nonblocking.tokens Require Import logrel_tok tokens_ra.
 
 
 From trillium.program_logic Require Import weakestpre. 
 From heap_lang Require Import heap_lang_defs lang notation.
 From lawyer.obligations Require Import obligations_resources.
 
-
-From iris.algebra Require Import excl. 
-Class MethodTokenPre Σ := {
-    ut_pre_tok :: inG Σ (exclR positive);
-}.
-Class MethodToken Σ := {
-    ut_pre_pre :: MethodTokenPre Σ;
-    ut_γ: gname;
-}.
-Definition method_tok `{MethodToken Σ} (v: val) :=
- own ut_γ (Excl $ encode v).
-
-Definition methods_restr := gmap val nat.
-
 Definition method_spec_token {M} {EM: ExecutionModel heap_lang M} {Σ} {OHE: OM_HL_Env OP_HL_WF EM Σ}
-  {MT: MethodToken Σ}
+  MS {MT: MethodToken MS Σ}
     F (m: val): iProp Σ := 
   ∀ τ π q (a: val),
     {{{ cp_mul π d_wfr0 F ∗ th_phase_frag τ π q ∗ method_tok m }}}
@@ -33,7 +19,7 @@ Definition method_spec_token {M} {EM: ExecutionModel heap_lang M} {Σ} {OHE: OM_
 
 
 (** TODO: add the stuckness bit? *)
-Record WaitFreeSpecToken (ms: methods_restr) := {
+Record WaitFreeSpecToken (MS: gmultiset val) := {
   wfst_is_init_st: cfg heap_lang -> Prop;
   (** for wait-free modules, we expect that invariant doesn't contain OM resources *)
   wfst_mod_inv {Σ} {hG: heap1GS Σ} {iG: invGS_gen HasNoLc Σ}: iProp Σ;
@@ -42,15 +28,15 @@ Record WaitFreeSpecToken (ms: methods_restr) := {
   wfst_init_mod `{heap1GS Σ, invGS_gen HasNoLc Σ, MethodTokenPre Σ}:
     forall c (INIT: wfst_is_init_st c),
       ⊢ hl_phys_init_resource c ={⊤}=∗ wfst_mod_inv ∗ 
-          ∃ (_: MethodToken Σ), ([∗ map] m ↦ k ∈ ms, [∗] replicate k (method_tok m));
+          ∃ (_: MethodToken MS Σ), methods_toks MS;
   wfst_F: nat;
   wfst_spec:
   forall {M: Model} {EM: ExecutionModel heap_lang M} {Σ} {OHE: OM_HL_Env OP_HL_WF EM Σ}
-    {MT: MethodToken Σ},
+    {MT: MethodToken MS Σ},
     (let _: heap1GS Σ := iem_phys HeapLangEM EM in wfst_mod_inv) ⊢
-    [∗ set] m ∈ dom ms, method_spec_token wfst_F m;
+    [∗ set] m ∈ dom MS, method_spec_token MS wfst_F m;
     
   wfst_safety_spec:
-    ∀ {Σ : gFunctors} `{heap1GS Σ, invGS_gen HasNoLc Σ, MethodToken Σ},
-      wfst_mod_inv ⊢ [∗ set] m ∈ dom ms, interp (method_tok m) si_add_none m;
+    ∀ {Σ : gFunctors} `{heap1GS Σ, invGS_gen HasNoLc Σ, MethodToken MS Σ},
+      wfst_mod_inv ⊢ [∗ set] m ∈ dom MS, interp (method_tok m) si_add_none m;
 }.
