lawyer/nonblocking/tokens/tokens_ra.v
@@ -1,0 +1,46 @@
+From iris.proofmode Require Import tactics.
+From iris.algebra Require Import gmultiset.
+From heap_lang Require Import lang.
+
+
+Class MethodTokenPre (Σ: gFunctors) := {
+    (* mt_pre_tok :: inG Σ (exclR positive); *)
+}.
+Class MethodToken (MS: gmultiset val) (Σ: gFunctors) := {
+    (* ut_pre_pre :: MethodTokenPre Σ; *)
+    mt_γ: gname;
+}.
+
+
+(* TODO: generalize, upstream *)
+Section TokensRA.
+  Context `{MethodToken MS Σ}.
+  
+  Definition methods_toks (ms: gmultiset val): iProp Σ. Admitted.
+
+  (* Global Instance is_op_mt m1 m2 :  *)
+  (*   IsOp (methods_toks (m1 ⊎ m2)) (methods_toks m1) (methods_toks m2). *)
+  (* Proof. by rewrite /IsOp' /IsOp frac_op Qp.div_2. Qed. *)
+
+  Lemma methods_toks_split ms1 ms2:
+    methods_toks (ms1 ⊎ ms2) ⊣⊢ methods_toks ms1 ∗ methods_toks ms2.
+  Proof using. Admitted.
+
+  Lemma methods_toks_sub ms:
+    methods_toks ms -∗ ⌜ ms ⊆ MS ⌝.
+  Proof using. Admitted. 
+
+  Definition method_tok (m: val) := methods_toks {[+ m +]}. 
+
+  Lemma method_tok_sub m:
+    method_tok m -∗ ⌜ m ∈ MS ⌝.
+  Proof using.
+    rewrite -gmultiset_singleton_subseteq_l. 
+    iApply methods_toks_sub.
+  Qed.  
+
+End TokensRA.
+
+Lemma mt_init `{MethodTokenPre Σ} MS:
+  ⊢ ∃ (MT: MethodToken MS Σ), methods_toks MS.
+Proof using. Admitted.
